\section{Triangle Count Estimation}

\subsection{Expected Value of $\alpha$}

Consider a triangle in $G$. WLOG, let $u$ and $v$ be the vertices picked by the algorithm as an edge $e = \{u, v\}$ and $w$ is picked from the remaining vertices. In reality, any two vertices of the three forming this triangle can be picked as an edge first. The probability that the algorithm picks this triangle is
\begin{equation*}
\begin{aligned}
  & \text{$\#$ edges in triangle} \cdot
    \text{$\mathbf{Pr}$[Picking $e = \{u, v\}$]} \cdot
    \text{$\mathbf{Pr}$[Picking $w$ from $V\backslash\{u, v\}$]} \\
  =\quad & 3 \cdot \frac{1}{m} \cdot \frac{1}{n-2} \\
  =\quad & \frac{3}{m(n-2)}
\end{aligned}
\end{equation*}

Since there are $\tau$ triangles in $G$, we have that the probability of the algorithm picking any triangle is 
\[
  \mathbf{Pr}[\text{Algorithm picks a triangle}] = \frac{3}{m(n-2)} \cdot \tau
\]

Recall the definition of $\alpha$
\[
  \alpha \begin{cases}
    1 & \text{if the algorithm picks a triangle} \\
    0 & \text{otherwise}
  \end{cases}
\]
Therefore, 
\begin{equation*}
\begin{aligned}
  \mathbf{E}[\alpha]
    &= 1 \cdot \mathbf{Pr}[\text{Algorithm picks a triangle}] + 0 \cdot \mathbf{Pr}[\text{Algorithm doesn't pick a triangle}] \\
    &= 1 \cdot \frac{3\tau}{m(n-2)} + 0 \cdot \left(1 - \frac{3\tau}{m(n-2)}\right) \\
  \therefore \mathbf{E}[\alpha]
    &= \frac{3\tau}{m(n-2)} \quad \qedsymbol
\end{aligned}
\end{equation*}

\subsection{Expected Value of $\hat{\tau}$}

Consider
\begin{equation*}
\begin{aligned}
  \hat{\tau}
    &= \frac{m(n-2)}{3}\cdot\hat{\alpha} \\
  \mathbf{E}[\hat{\tau}]
    &= \mathbf{E}\left[\frac{m(n-2)}{3}\cdot\hat{\alpha}\right] \\
    &= \frac{m(n-2)}{3}\cdot\mathbf{E}\left[\hat{\alpha}\right] \quad \text{($m$ and $n$ are not random)} \\
    &= \frac{m(n-2)}{3}\cdot\mathbf{E}\left[\frac{1}{T}\left(\alpha_1 + \alpha_2 + \cdots + \alpha_T\right)\right] \\
    &= \frac{m(n-2)}{3}\cdot\frac{1}{T}\left(\mathbf{E}[\alpha_1] + \mathbf{E}[\alpha_2] + \cdots + \mathbf{E}[\alpha_T]\right) \\
    &= \frac{m(n-2)}{3}\cdot\frac{1}{T}\left(\sum_{i=1}^T \mathbf{E}[\alpha]\right) \\
    &= \frac{m(n-2)}{3}\cdot\frac{T}{T}\cdot \frac{3\tau}{m(n-2)} \\
  \therefore \mathbf{E}[\hat{\tau}]
    &= \tau \quad \qedsymbol
\end{aligned}
\end{equation*}

\subsection{Finding a $T$}

